Prove an alternative (equivalent) statement for transition.safe
...assuming the relation is determinist.
Hopefully the alternative statement is more easy to use.

verified/transition.lean
@@ -10,6 +10,7 @@ structure system (label : Type v) :=
     (step : state → state → list label → Prop)
     (init : state)
     (final : state → Prop)
+    (step_final : ∀ s s' ls, final s → ¬ (step s s' ls))
 
 -- FIXME
 -- instance : has_coe system Type := ⟨system.state⟩
@@ -18,6 +19,12 @@ section sequences
 
 variable {α : Type u}
 variable {label : Type v}
+
+def determinist (R : α → α → list label → Prop) :=
+  ∀ s s1 s2 ls1 ls2,
+  R s s1 ls1 →
+  R s s2 ls2 →
+  s1 = s2 ∧ ls1 = ls2
 
 inductive star (R : α → α → list label → Prop) : α → α → list label → Prop
 | refl : ∀ a,
@@ -86,6 +93,64 @@ def safe {lbl} (sys : system lbl) :=
   ∀ s ls,
     (star sys.step) sys.init s ls →
     unstuck sys s
+
+lemma safe_step {lbl} (sys : system lbl) :
+  safe sys → sys.final sys.init ∨ (∃ s' ls, sys.step sys.init s' ls ∧ safe {sys with init := s'})
+:=
+begin
+  intro S, /- simp [safe] at S -/ --FIXME
+  unfold safe at S,
+  note S0 := S sys.init [] (by { constructor }), unfold unstuck at S0,
+  cases S0 with _ S'; [left, right], --[ {left, assumption} , skip ],
+  { assumption },
+  { cases S' with s' S', cases S' with ls S', existsi [_, _], split, -- FIXME?
+    assumption,
+    simp [safe], dsimp, intros s'' ls' S'',
+    apply S, constructor; assumption
+  }
+end
+
+lemma step_safe {lbl} (sys : system lbl) :
+  determinist sys.step →
+  sys.final sys.init ∨ (∃ s' ls, sys.step sys.init s' ls ∧ safe {sys with init := s'}) → safe sys
+:=
+begin
+  assert step_safe' : ∀ {T} (init : T) (step : T → T → list lbl → Prop) sf lsf,
+    determinist step →
+    (star step) init sf lsf →
+    ∀ (final : T → Prop) step_final,
+      (final init ∨ (∃ s' ls, step init s' ls ∧ safe (system.mk T step s' final step_final))) →
+      unstuck (system.mk T step init final step_final) sf,
+  { introv D SS, induction SS,
+    case star.refl {
+      intro H, simp [unstuck], cases H with _ H; [left, right], assumption,
+      cases H with _ H, cases H with _ H, cases H, existsi [_, _], assumption
+    },
+
+    case star.step s0 s1 s2 ls1 ls2 S1 S2 IH {
+      intro H,
+      cases H with H H, { cases (step_final _ _ _ H S1) },
+      cases H with s1' H, cases H with ls1' H, cases H with S1' Hs1',
+      cases (D _ _ _ _ _ S1 S1') with e1 e2, subst e1, subst e2, clear S1',
+      note HS1'' := safe_step _ Hs1', dsimp at HS1'',
+      note IH' := IH HS1'', clear IH, /- FIXME specialize -/
+      apply IH'
+    }
+  },
+
+  intros D H s ls SS, cases sys, dsimp at *, apply step_safe'; assumption
+end
+
+lemma safe_step_iff {lbl} (sys : system lbl) :
+  determinist sys.step →
+  (safe sys ↔ sys.final sys.init ∨ (∃ s' ls, sys.step sys.init s' ls ∧ safe {sys with init := s'}))
+:=
+begin
+  intro,
+  split; intro,
+  { apply safe_step; assumption },
+  { apply step_safe; assumption }
+end
 
 def quasi_refinement
   {lbl} (A B : system lbl) (R : A.state → B.state → Prop) :
